Refactor `heaplang/opsem_adequacy.v` so that it relies on `heaplang/adequacy.v`.

src/heaplang/opsem_adequacy.v
@@ -6,9 +6,9 @@ From ITree Require Import ITree Recursion RecursionFacts InterpFacts Eqit.
 From iris.program_logic Require Import language.
 (* TODO: make the import order less brittle *)
 From iris.itree.heaplang Require Import decide.
-From iris.itree Require Import later handler.
+From iris.itree Require Import later handler void.
 From iris.itree.threadpool Require Import handler interleaving.
-From iris.itree.heaplang Require Import lang.
+From iris.itree.heaplang Require Import lang adequacy.
 From Paco Require Import paco.
 From Paco Require Import paco2.
 
@@ -78,7 +78,7 @@ Qed.
 Lemma base_Beta f_ x_ e v :
   compile_expr (App (Val (RecV f_ x_ e)) (Val v))
   ≈ let e' := (subst' x_ v (subst' f_ (RecV f_ x_ e) e))
-     in step_if_not_val e' ;; yield_if_not_val e' ;; compile_expr e'.
+     in step ;; yield_if_not_val e' ;; compile_expr e'.
 Proof.
   rewrite /compile_expr. eutt_norm/=. setoid_rewrite interp_recursive_call. by eutt_norm/=.
 Qed.
@@ -422,33 +422,9 @@ Proof.
         apply Hstuck. exists tid, e'. eauto.
 Qed.
 
-Variant Terminal (R : Type) :=
-  | TermRet (r : R)
-  | TermUb.
-Global Arguments TermRet {_}.
-Global Arguments TermUb {_}.
-Definition terminal_trace {E R} `{ubE -< E} (tx : Terminal R) : trace E R :=
-  match tx with
-  | TermRet r => TRet r
-  | TermUb => TVisEmpty void (subevent _ EUb)
-  end.
-Definition terminal_ctrace {E R} `{ubE -< E} (tx : Terminal R) : ctrace E R :=
-  match tx with
-  | TermRet r => CTRet r
-  | TermUb => CTVisEmpty void (subevent _ EUb)
-  end.
-
-Instance Terminal_FMap : FMap Terminal :=
-  λ _ _ f tx,
-    match tx with
-    | TermRet r => TermRet (f r)
-    | TermUb => TermUb
-    end.
-
-Definition trace_terminates_in {E R} `{ubE -< E} (tr : trace E R) (tx : Terminal R) :=
-  is_postfix (terminal_trace tx) tr.
-Definition ctrace_terminates_in {E R} `{ubE -< E} (tr : ctrace E R) (tx : Terminal R) :=
-  is_postfix_ctrace (terminal_ctrace tx) tr.
+Definition Terminal (R : Type) : Type := R + ub_crash.
+Notation TermUb := (inr UbCrash).
+Notation TermRet r := (inl r).
 
 Variant tp_termination : list expr → state → Terminal val → Prop :=
   | tp_termination_TermUb tp σ :
@@ -457,28 +433,20 @@ Variant tp_termination : list expr → state → Terminal val → Prop :=
   | tp_termination_TermRet v tp σ :
     tp_termination (Val v :: tp) σ (TermRet v).
 
+Definition tr_terminal (tx : Terminal val) (tr : trace voidE (state * (val + last_thread_killed) + later_exhausted + ub_crash)) : bool :=
+  match tx, tr with
+  | TermUb, TRet (inr UbCrash) => true
+  | TermRet r, TRet (inl (inl (_, (inl r')))) => bool_decide (r = r')
+  | _, _ => false
+  end.
+
 (* TODO: Factor this event type into its own definition. *)
-Definition trace_invariant_postfix (tx : Terminal val) (tr : ctrace (demonicE +' stateE state +' laterE +' ubE) val) :=
-  ctrace_terminates_in tr tx.
-Definition trace_invariant_state σ (tr : ctrace (demonicE +' stateE state +' laterE +' ubE) val) :=
+Definition trace_invariant σ (tx : Terminal val) (opsem_steps : nat) (tr : ctrace (demonicE +' stateE state +' laterE +' ubE) val) :=
   match (interp_tr_state σ (interp_tr (sequencify tr))) with
-  | Some _ => true
+  | Some tr => tr_terminal tx (interp_tr_ub (insert_voidE_tr (interp_tr_later (Some opsem_steps) tr)))
   | None => false
   end.
-(* TODO: Add invariant about the final state reached in trace. Should be σ'. *)
-Definition trace_invariant σ (tx : Terminal val) (tr : ctrace (demonicE +' stateE state +' laterE +' ubE) val) :=
-  trace_invariant_postfix tx tr ∧
-  trace_invariant_state σ tr.
-
-Lemma trace_invariant_postfix_postfix tx tr tr' :
-  is_postfix_ctrace tr tr' →
-  trace_invariant_postfix tx tr →
-  trace_invariant_postfix tx tr'.
-Proof.
-  intros Hpost Htinv. rewrite /trace_invariant_postfix/ctrace_terminates_in.
-  rewrite /trace_invariant_postfix/ctrace_terminates_in in Htinv.
-  by etransitivity.
-Qed.
+Arguments trace_invariant _ _ / _ _.
 
 Lemma tp_termination_ub (tp : list expr) (σ : state) :
   tp_termination tp σ TermUb →
@@ -495,13 +463,12 @@ Proof.
   exists (Ret v). split; first done. constructor.
 Qed.
 
-Lemma trace_invariant_ret tp σ v :
+Lemma trace_invariant_ret tp σ n v :
   tp_termination tp σ (TermRet v) →
-  trace_invariant σ (TermRet v) (CTRet v).
+  trace_invariant σ (TermRet v) n (CTRet v).
 Proof.
   intros Hterm. inversion Hterm. subst.
-  split; last done.
-  constructor.
+  by apply bool_decide_pack.
 Qed.
 
 Lemma UnOp_stuck op v σ :
@@ -558,21 +525,21 @@ Proof.
   by rewrite list_insert_insert.
 Qed.
 
-Lemma state_invariant_yield tid σ tr :
-  trace_invariant_state σ tr →
-  trace_invariant_state σ (CTYield tid tr).
+Lemma trace_invariant_yield tid σ n tx tr :
+  trace_invariant σ tx n tr →
+  trace_invariant σ tx n (CTYield tid tr).
 Proof.
   intros Hinv.
-  rewrite /trace_invariant_state. rewrite /trace_invariant_state in Hinv.
+  rewrite /trace_invariant. rewrite /trace_invariant in Hinv.
   rewrite /ctrace_step_yield /=. by destruct (interp_tr_state _ _).
 Qed.
 
-Lemma state_invariant_step_yield tid σ tr :
-  trace_invariant_state σ tr →
-  trace_invariant_state σ (ctrace_step_yield tid tr).
+Lemma trace_invariant_step_yield tid σ tx n tr :
+  trace_invariant σ tx n tr →
+  trace_invariant σ tx (S n) (ctrace_step_yield tid tr).
 Proof.
   intros Hinv.
-  rewrite /trace_invariant_state. rewrite /trace_invariant_state in Hinv.
+  rewrite /trace_invariant. rewrite /trace_invariant in Hinv.
   rewrite /ctrace_step_yield /=. by destruct (interp_tr_state _ _).
 Qed.
 
@@ -672,32 +639,32 @@ Proof.
     { rewrite list_lookup_insert //. by apply lookup_lt_is_Some. }
 Qed.
 
-Lemma state_invariant_store' l x σ tr :
-  trace_invariant_state (state_upd_heap <[l:=x]> σ) tr →
-  trace_invariant_state σ (ctrace_store' l x σ tr).
+Lemma trace_invariant_store' l x σ tx n tr :
+  trace_invariant (state_upd_heap <[l:=x]> σ) tx n tr →
+  trace_invariant σ tx n (ctrace_store' l x σ tr).
 Proof.
   intros Hinv.
-  rewrite /trace_invariant_state. rewrite /trace_invariant_state in Hinv.
+  rewrite /trace_invariant. rewrite /trace_invariant in Hinv.
   simpl. rewrite decide_True //.
 Qed.
-Lemma state_invariant_store l x σ tr :
-  trace_invariant_state (state_upd_heap <[l:=Some x]> σ) tr →
-  trace_invariant_state σ (ctrace_store l x σ tr).
+Lemma trace_invariant_store l x σ tx n tr :
+  trace_invariant (state_upd_heap <[l:=Some x]> σ) tx n tr →
+  trace_invariant σ tx n (ctrace_store l x σ tr).
 Proof.
-  intros Hinv. by apply state_invariant_store'.
+  intros Hinv. by apply trace_invariant_store'.
 Qed.
-Lemma state_invariant_load σ tr :
-  trace_invariant_state σ tr →
-  trace_invariant_state σ (ctrace_load σ tr).
+Lemma trace_invariant_load σ tx n tr :
+  trace_invariant σ tx n tr →
+  trace_invariant σ tx n (ctrace_load σ tr).
 Proof.
   intros Hinv.
-  rewrite /trace_invariant_state. rewrite /trace_invariant_state in Hinv.
+  rewrite /trace_invariant. rewrite /trace_invariant in Hinv.
   simpl. rewrite decide_True //.
 Qed.
 
 Lemma stuck_ub tp σ :
   tp_termination tp σ TermUb →
-  ∃ tid tr, trace_invariant σ TermUb tr ∧ is_ctrace tr tid (compile_tp tp).
+  ∃ tid tr, trace_invariant σ TermUb 0 tr ∧ is_ctrace tr tid (compile_tp tp).
 Proof.
   intros Hterm.
   assert (Hterm' := Hterm).
@@ -705,9 +672,7 @@ Proof.
   exists tid.
   destruct Hbasic as [x|f x e0|v1 v2 | | | | | | | | | | | | | | | | | | ].
   - exists ctrace_ub.
-    split; first split.
-    { constructor. }
-    { done. }
+    split; first done.
     eapply is_ctrace_insert.
     { rewrite /compile_tp list_lookup_fmap enumerate_lookup' Htp //. }
     { rewrite /compile_expr_yield compile_expr_bind'; first done. admit. }
@@ -718,9 +683,7 @@ Proof.
     eapply Ectx_step with (K := []); eauto.
     by constructor.
   - exists ctrace_ub.
-    split; first split.
-    { constructor. }
-    { done. }
+    split; first done.
     eapply is_ctrace_insert.
     { rewrite /compile_tp list_lookup_fmap enumerate_lookup' Htp //. }
     { rewrite /compile_expr_yield compile_expr_bind'; first done. admit. }
@@ -733,9 +696,7 @@ Proof.
       eapply is_ctrace_ub.
       rewrite list_lookup_insert // compile_tp_len -lookup_lt_is_Some //.
   - exists ctrace_ub.
-    split; first split.
-    { constructor. }
-    { done. }
+    split; first done.
     eapply is_ctrace_insert.
     { rewrite /compile_tp list_lookup_fmap enumerate_lookup' Htp //. }
     { rewrite /compile_expr_yield compile_expr_bind'; first done. admit. }
@@ -744,9 +705,7 @@ Proof.
     is_ctrace_norm/=. eapply is_ctrace_ub.
     rewrite list_lookup_insert // compile_tp_len -lookup_lt_is_Some //.
   - exists ctrace_ub.
-    split; first split.
-    { constructor. }
-    { done. }
+    split; first done.
     eapply is_ctrace_insert.
     { rewrite /compile_tp list_lookup_fmap enumerate_lookup' Htp //. }
     { rewrite /compile_expr_yield compile_expr_bind'; first done. admit. }
@@ -755,9 +714,7 @@ Proof.
     is_ctrace_norm/=. eapply is_ctrace_ub.
     rewrite list_lookup_insert // compile_tp_len -lookup_lt_is_Some //.
   - exists ctrace_ub.
-    split; first split.
-    { constructor. }
-    { done. }
+    split; first done.
     eapply is_ctrace_insert.
     { rewrite /compile_tp list_lookup_fmap enumerate_lookup' Htp //. }
     { rewrite /compile_expr_yield compile_expr_bind'; first done. admit. }
@@ -774,9 +731,7 @@ Proof.
     eapply Ectx_step with (K := []); eauto.
     by constructor.
   - exists ctrace_ub.
-    split; first split.
-    { constructor. }
-    { done. }
+    split; first done.
     eapply is_ctrace_insert.
     { rewrite /compile_tp list_lookup_fmap enumerate_lookup' Htp //. }
     { rewrite /compile_expr_yield compile_expr_bind'; first done. admit. }
@@ -789,9 +744,7 @@ Proof.
       eapply is_ctrace_ub.
       rewrite list_lookup_insert // compile_tp_len -lookup_lt_is_Some //.
   - exists ctrace_ub.
-    split; first split.
-    { constructor. }
-    { done. }
+    split; first done.
     eapply is_ctrace_insert.
     { rewrite /compile_tp list_lookup_fmap enumerate_lookup' Htp //. }
     { rewrite /compile_expr_yield compile_expr_bind'; first done. admit. }
@@ -810,9 +763,7 @@ Proof.
     eapply Ectx_step with (K := []); eauto.
     by constructor.
   - exists ctrace_ub.
-    split; first split.
-    { constructor. }
-    { done. }
+    split; first done.
     eapply is_ctrace_insert.
     { rewrite /compile_tp list_lookup_fmap enumerate_lookup' Htp //. }
     { rewrite /compile_expr_yield compile_expr_bind'; first done. admit. }
@@ -832,9 +783,7 @@ Proof.
     eapply Ectx_step with (K := []); eauto.
     by constructor.
   - exists ctrace_ub.
-    split; first split.
-    { constructor. }
-    { done. }
+    split; first done.
     eapply is_ctrace_insert.
     { rewrite /compile_tp list_lookup_fmap enumerate_lookup' Htp //. }
     { rewrite /compile_expr_yield compile_expr_bind'; first done. admit. }
@@ -861,29 +810,23 @@ Proof.
         eapply Ectx_step with (K := []); eauto.
         by eapply FreeS.
       + exists (ctrace_store'_ub σ).
-        split; first split.
-        ++ repeat constructor.
-        ++ rewrite /trace_invariant_state /= decide_True //.
-        ++ eapply is_ctrace_insert.
-           { rewrite /compile_tp list_lookup_fmap enumerate_lookup' Htp //. }
-           { rewrite /compile_expr_yield compile_expr_bind'; first done. admit. }
-           rewrite /compile_expr. is_ctrace_norm/=. rewrite Heq /=. is_ctrace_norm/=.
-           eapply is_ctrace_store'_ub; first by left.
-           { rewrite list_lookup_insert // compile_tp_len -lookup_lt_is_Some //. }
+        split; first rewrite /= decide_True //.
+        eapply is_ctrace_insert.
+        { rewrite /compile_tp list_lookup_fmap enumerate_lookup' Htp //. }
+        { rewrite /compile_expr_yield compile_expr_bind'; first done. admit. }
+        rewrite /compile_expr. is_ctrace_norm/=. rewrite Heq /=. is_ctrace_norm/=.
+        eapply is_ctrace_store'_ub; first by left.
+        { rewrite list_lookup_insert // compile_tp_len -lookup_lt_is_Some //. }
       + exists (ctrace_store'_ub σ).
-        split; first split.
-        ++ repeat constructor.
-        ++ rewrite /trace_invariant_state /= decide_True //.
-        ++ eapply is_ctrace_insert.
-           { rewrite /compile_tp list_lookup_fmap enumerate_lookup' Htp //. }
-           { rewrite /compile_expr_yield compile_expr_bind'; first done. admit. }
-           rewrite /compile_expr. is_ctrace_norm/=. rewrite Heq /=. is_ctrace_norm/=.
-           eapply is_ctrace_store'_ub; first by right.
-           { rewrite list_lookup_insert // compile_tp_len -lookup_lt_is_Some //. }
+        split; first rewrite /= decide_True //.
+        eapply is_ctrace_insert.
+        { rewrite /compile_tp list_lookup_fmap enumerate_lookup' Htp //. }
+        { rewrite /compile_expr_yield compile_expr_bind'; first done. admit. }
+        rewrite /compile_expr. is_ctrace_norm/=. rewrite Heq /=. is_ctrace_norm/=.
+        eapply is_ctrace_store'_ub; first by right.
+        { rewrite list_lookup_insert // compile_tp_len -lookup_lt_is_Some //. }
     * exists ctrace_ub.
-      split; first split.
-      { constructor. }
-      { done. }
+      split; first done.
       eapply is_ctrace_insert.
       { rewrite /compile_tp list_lookup_fmap enumerate_lookup' Htp //. }
       { rewrite /compile_expr_yield compile_expr_bind'; first done. admit. }
@@ -899,29 +842,23 @@ Proof.
         eapply Ectx_step with (K := []); eauto.
         by eapply LoadS.
       + exists (ctrace_load_ub σ).
-        split; first split.
-        ++ repeat constructor.
-        ++ rewrite /trace_invariant_state /= decide_True //.
-        ++ eapply is_ctrace_insert.
-           { rewrite /compile_tp list_lookup_fmap enumerate_lookup' Htp //. }
-           { rewrite /compile_expr_yield compile_expr_bind'; first done. admit. }
-           rewrite /compile_expr. is_ctrace_norm/=. rewrite Heq /=. is_ctrace_norm/=.
-           eapply is_ctrace_load_ub; first by left.
-           { rewrite list_lookup_insert // compile_tp_len -lookup_lt_is_Some //. }
+        split; first rewrite /= decide_True //.
+        eapply is_ctrace_insert.
+        { rewrite /compile_tp list_lookup_fmap enumerate_lookup' Htp //. }
+        { rewrite /compile_expr_yield compile_expr_bind'; first done. admit. }
+        rewrite /compile_expr. is_ctrace_norm/=. rewrite Heq /=. is_ctrace_norm/=.
+        eapply is_ctrace_load_ub; first by left.
+        { rewrite list_lookup_insert // compile_tp_len -lookup_lt_is_Some //. }
       + exists (ctrace_load_ub σ).
-        split; first split.
-        ++ repeat constructor.
-        ++ rewrite /trace_invariant_state /= decide_True //.
-        ++ eapply is_ctrace_insert.
-           { rewrite /compile_tp list_lookup_fmap enumerate_lookup' Htp //. }
-           { rewrite /compile_expr_yield compile_expr_bind'; first done. admit. }
-           rewrite /compile_expr. is_ctrace_norm/=. rewrite Heq /=. is_ctrace_norm/=.
-           eapply is_ctrace_load_ub; first by right.
-           { rewrite list_lookup_insert // compile_tp_len -lookup_lt_is_Some //. }
+        split; first rewrite /= decide_True //.
+        eapply is_ctrace_insert.
+        { rewrite /compile_tp list_lookup_fmap enumerate_lookup' Htp //. }
+        { rewrite /compile_expr_yield compile_expr_bind'; first done. admit. }
+        rewrite /compile_expr. is_ctrace_norm/=. rewrite Heq /=. is_ctrace_norm/=.
+        eapply is_ctrace_load_ub; first by right.
+        { rewrite list_lookup_insert // compile_tp_len -lookup_lt_is_Some //. }
     * exists ctrace_ub.
       split; first split.
-      { constructor. }
-      { done. }
       eapply is_ctrace_insert.
       { rewrite /compile_tp list_lookup_fmap enumerate_lookup' Htp //. }
       { rewrite /compile_expr_yield compile_expr_bind'; first done. admit. }
@@ -937,29 +874,23 @@ Proof.
         eapply Ectx_step with (K := []); eauto.
         by eapply StoreS.
       + exists (ctrace_store_ub σ).
-        split; first split.
-        ++ repeat constructor.
-        ++ rewrite /trace_invariant_state /= decide_True //.
-        ++ eapply is_ctrace_insert.
-           { rewrite /compile_tp list_lookup_fmap enumerate_lookup' Htp //. }
-           { rewrite /compile_expr_yield compile_expr_bind'; first done. admit. }
-           rewrite /compile_expr. is_ctrace_norm/=. rewrite Heq /=. is_ctrace_norm/=.
-           eapply is_ctrace_store_ub; first by left.
-           { rewrite list_lookup_insert // compile_tp_len -lookup_lt_is_Some //. }
+        split; first rewrite /= decide_True //.
+        eapply is_ctrace_insert.
+        { rewrite /compile_tp list_lookup_fmap enumerate_lookup' Htp //. }
+        { rewrite /compile_expr_yield compile_expr_bind'; first done. admit. }
+        rewrite /compile_expr. is_ctrace_norm/=. rewrite Heq /=. is_ctrace_norm/=.
+        eapply is_ctrace_store_ub; first by left.
+        { rewrite list_lookup_insert // compile_tp_len -lookup_lt_is_Some //. }
       + exists (ctrace_store_ub σ).
-        split; first split.
-        ++ repeat constructor.
-        ++ rewrite /trace_invariant_state /= decide_True //.
-        ++ eapply is_ctrace_insert.
-           { rewrite /compile_tp list_lookup_fmap enumerate_lookup' Htp //. }
-           { rewrite /compile_expr_yield compile_expr_bind'; first done. admit. }
-           rewrite /compile_expr. is_ctrace_norm/=. rewrite Heq /=. is_ctrace_norm/=.
-           eapply is_ctrace_store_ub; first by right.
-           { rewrite list_lookup_insert // compile_tp_len -lookup_lt_is_Some //. }
+        split; first rewrite /= decide_True //.
+        eapply is_ctrace_insert.
+        { rewrite /compile_tp list_lookup_fmap enumerate_lookup' Htp //. }
+        { rewrite /compile_expr_yield compile_expr_bind'; first done. admit. }
+        rewrite /compile_expr. is_ctrace_norm/=. rewrite Heq /=. is_ctrace_norm/=.
+        eapply is_ctrace_store_ub; first by right.
+        { rewrite list_lookup_insert // compile_tp_len -lookup_lt_is_Some //. }
     * exists ctrace_ub.
-      split; first split.
-      { constructor. }
-      { done. }
+      split; first done.
       eapply is_ctrace_insert.
       { rewrite /compile_tp list_lookup_fmap enumerate_lookup' Htp //. }
       { rewrite /compile_expr_yield compile_expr_bind'; first done. admit. }
@@ -975,29 +906,23 @@ Proof.
         eapply Ectx_step with (K := []); eauto.
         by eapply XchgS.
       + exists (ctrace_store_ub σ).
-        split; first split.
-        ++ repeat constructor.
-        ++ rewrite /trace_invariant_state /= decide_True //.
-        ++ eapply is_ctrace_insert.
-           { rewrite /compile_tp list_lookup_fmap enumerate_lookup' Htp //. }
-           { rewrite /compile_expr_yield compile_expr_bind'; first done. admit. }
-           rewrite /compile_expr. is_ctrace_norm/=. rewrite Heq /=. is_ctrace_norm/=.
-           eapply is_ctrace_store_ub; first by left.
-           { rewrite list_lookup_insert // compile_tp_len -lookup_lt_is_Some //. }
+        split; first rewrite /= decide_True //.
+        eapply is_ctrace_insert.
+        { rewrite /compile_tp list_lookup_fmap enumerate_lookup' Htp //. }
+        { rewrite /compile_expr_yield compile_expr_bind'; first done. admit. }
+        rewrite /compile_expr. is_ctrace_norm/=. rewrite Heq /=. is_ctrace_norm/=.
+        eapply is_ctrace_store_ub; first by left.
+        { rewrite list_lookup_insert // compile_tp_len -lookup_lt_is_Some //. }
       + exists (ctrace_store_ub σ).
-        split; first split.
-        ++ repeat constructor.
-        ++ rewrite /trace_invariant_state /= decide_True //.
-        ++ eapply is_ctrace_insert.
-           { rewrite /compile_tp list_lookup_fmap enumerate_lookup' Htp //. }
-           { rewrite /compile_expr_yield compile_expr_bind'; first done. admit. }
-           rewrite /compile_expr. is_ctrace_norm/=. rewrite Heq /=. is_ctrace_norm/=.
-           eapply is_ctrace_store_ub; first by right.
-           { rewrite list_lookup_insert // compile_tp_len -lookup_lt_is_Some //. }
+        split; first rewrite /= decide_True //.
+        eapply is_ctrace_insert.
+        { rewrite /compile_tp list_lookup_fmap enumerate_lookup' Htp //. }
+        { rewrite /compile_expr_yield compile_expr_bind'; first done. admit. }
+        rewrite /compile_expr. is_ctrace_norm/=. rewrite Heq /=. is_ctrace_norm/=.
+        eapply is_ctrace_store_ub; first by right.
+        { rewrite list_lookup_insert // compile_tp_len -lookup_lt_is_Some //. }
     * exists ctrace_ub.
-      split; first split.
-      { constructor. }
-      { done. }
+      split; first done.
       eapply is_ctrace_insert.
       { rewrite /compile_tp list_lookup_fmap enumerate_lookup' Htp //. }
       { rewrite /compile_expr_yield compile_expr_bind'; first done. admit. }
@@ -1014,42 +939,34 @@ Proof.
            eapply Ectx_step with (K := []); eauto.
            by eapply CmpXchgS.
         ++ exists (ctrace_load σ ctrace_ub).
-           split; first split.
-           +++ repeat constructor.
-           +++ rewrite /trace_invariant_state /= decide_True //.
-           +++ eapply is_ctrace_insert.
-               { rewrite /compile_tp list_lookup_fmap enumerate_lookup' Htp //. }
-               { rewrite /compile_expr_yield compile_expr_bind'; first done. admit. }
-               rewrite /compile_expr. is_ctrace_norm/=. rewrite Heq /=. is_ctrace_norm/=.
-               eapply is_ctrace_load; first done.
-               { rewrite list_lookup_insert // compile_tp_len -lookup_lt_is_Some //. }
-               is_ctrace_norm/=. rewrite assert_False // /ub.
-               eapply is_ctrace_ub.
-               rewrite list_lookup_insert // insert_length compile_tp_len -lookup_lt_is_Some //.
-      + exists (ctrace_load_ub σ).
-        split; first split.
-        ++ repeat constructor.
-        ++ rewrite /trace_invariant_state /= decide_True //.
-        ++ eapply is_ctrace_insert.
+           split; first rewrite /= decide_True //.
+           eapply is_ctrace_insert.
            { rewrite /compile_tp list_lookup_fmap enumerate_lookup' Htp //. }
            { rewrite /compile_expr_yield compile_expr_bind'; first done. admit. }
            rewrite /compile_expr. is_ctrace_norm/=. rewrite Heq /=. is_ctrace_norm/=.
-           eapply is_ctrace_load_ub; first by left.
+           eapply is_ctrace_load; first done.
            { rewrite list_lookup_insert // compile_tp_len -lookup_lt_is_Some //. }
+           is_ctrace_norm/=. rewrite assert_False // /ub.
+           eapply is_ctrace_ub.
+           rewrite list_lookup_insert // insert_length compile_tp_len -lookup_lt_is_Some //.
       + exists (ctrace_load_ub σ).
-        split; first split.
-        ++ repeat constructor.
-        ++ rewrite /trace_invariant_state /= decide_True //.
-        ++ eapply is_ctrace_insert.
-           { rewrite /compile_tp list_lookup_fmap enumerate_lookup' Htp //. }
-           { rewrite /compile_expr_yield compile_expr_bind'; first done. admit. }
-           rewrite /compile_expr. is_ctrace_norm/=. rewrite Heq /=. is_ctrace_norm/=.
-           eapply is_ctrace_load_ub; first by right.
-           { rewrite list_lookup_insert // compile_tp_len -lookup_lt_is_Some //. }
+        split; first rewrite /= decide_True //.
+        eapply is_ctrace_insert.
+        { rewrite /compile_tp list_lookup_fmap enumerate_lookup' Htp //. }
+        { rewrite /compile_expr_yield compile_expr_bind'; first done. admit. }
+        rewrite /compile_expr. is_ctrace_norm/=. rewrite Heq /=. is_ctrace_norm/=.
+        eapply is_ctrace_load_ub; first by left.
+        { rewrite list_lookup_insert // compile_tp_len -lookup_lt_is_Some //. }
+      + exists (ctrace_load_ub σ).
+        split; first rewrite /= decide_True //.
+        eapply is_ctrace_insert.
+        { rewrite /compile_tp list_lookup_fmap enumerate_lookup' Htp //. }
+        { rewrite /compile_expr_yield compile_expr_bind'; first done. admit. }
+        rewrite /compile_expr. is_ctrace_norm/=. rewrite Heq /=. is_ctrace_norm/=.
+        eapply is_ctrace_load_ub; first by right.
+        { rewrite list_lookup_insert // compile_tp_len -lookup_lt_is_Some //. }
     * exists ctrace_ub.
-      split; first split.
-      { constructor. }
-      { done. }
+      split; first done.
       eapply is_ctrace_insert.
       { rewrite /compile_tp list_lookup_fmap enumerate_lookup' Htp //. }
       { rewrite /compile_expr_yield compile_expr_bind'; first done. admit. }
@@ -1071,42 +988,34 @@ Proof.
                eapply Ectx_step with (K := []); eauto.
                by eapply FaaS.
            +++ exists (ctrace_load σ ctrace_ub).
-               split; first split.
-               ++++ repeat constructor.
-               ++++ rewrite /trace_invariant_state /= decide_True //.
-               ++++ eapply is_ctrace_insert.
-                    { rewrite /compile_tp list_lookup_fmap enumerate_lookup' Htp //. }
-                    { rewrite /compile_expr_yield compile_expr_bind'; first done. admit. }
-                    rewrite /compile_expr. is_ctrace_norm/=. rewrite Heq Heq' /=. is_ctrace_norm/=.
-                    eapply is_ctrace_load; first done.
-                    { rewrite list_lookup_insert // compile_tp_len -lookup_lt_is_Some //. }
-                    is_ctrace_norm/=. rewrite Heq''.
-                    eapply is_ctrace_ub.
-                    rewrite list_lookup_insert // insert_length compile_tp_len -lookup_lt_is_Some //.
-        ++ exists (ctrace_load_ub σ).
-           split; first split.
-           +++ repeat constructor.
-           +++ rewrite /trace_invariant_state /= decide_True //.
-           +++ eapply is_ctrace_insert.
+               split; first rewrite /= decide_True //.
+               eapply is_ctrace_insert.
                { rewrite /compile_tp list_lookup_fmap enumerate_lookup' Htp //. }
                { rewrite /compile_expr_yield compile_expr_bind'; first done. admit. }
                rewrite /compile_expr. is_ctrace_norm/=. rewrite Heq Heq' /=. is_ctrace_norm/=.
-               eapply is_ctrace_load_ub; first by left.
+               eapply is_ctrace_load; first done.
                { rewrite list_lookup_insert // compile_tp_len -lookup_lt_is_Some //. }
+               is_ctrace_norm/=. rewrite Heq''.
+               eapply is_ctrace_ub.
+               rewrite list_lookup_insert // insert_length compile_tp_len -lookup_lt_is_Some //.
         ++ exists (ctrace_load_ub σ).
-           split; first split.
-           +++ repeat constructor.
-           +++ rewrite /trace_invariant_state /= decide_True //.
-           +++ eapply is_ctrace_insert.
-               { rewrite /compile_tp list_lookup_fmap enumerate_lookup' Htp //. }
-               { rewrite /compile_expr_yield compile_expr_bind'; first done. admit. }
-               rewrite /compile_expr. is_ctrace_norm/=. rewrite Heq Heq' /=. is_ctrace_norm/=.
-               eapply is_ctrace_load_ub; first by right.
-               { rewrite list_lookup_insert // compile_tp_len -lookup_lt_is_Some //. }
+           split; first rewrite /= decide_True //.
+           eapply is_ctrace_insert.
+           { rewrite /compile_tp list_lookup_fmap enumerate_lookup' Htp //. }
+           { rewrite /compile_expr_yield compile_expr_bind'; first done. admit. }
+           rewrite /compile_expr. is_ctrace_norm/=. rewrite Heq Heq' /=. is_ctrace_norm/=.
+           eapply is_ctrace_load_ub; first by left.
+           { rewrite list_lookup_insert // compile_tp_len -lookup_lt_is_Some //. }
+        ++ exists (ctrace_load_ub σ).
+           split; first rewrite /= decide_True //.
+           eapply is_ctrace_insert.
+           { rewrite /compile_tp list_lookup_fmap enumerate_lookup' Htp //. }
+           { rewrite /compile_expr_yield compile_expr_bind'; first done. admit. }
+           rewrite /compile_expr. is_ctrace_norm/=. rewrite Heq Heq' /=. is_ctrace_norm/=.
+           eapply is_ctrace_load_ub; first by right.
+           { rewrite list_lookup_insert // compile_tp_len -lookup_lt_is_Some //. }
       + exists ctrace_ub.
-        split; first split.
-        { constructor. }
-        { done. }
+        split; first done.
         eapply is_ctrace_insert.
         { rewrite /compile_tp list_lookup_fmap enumerate_lookup' Htp //. }
         { rewrite /compile_expr_yield compile_expr_bind'; first done. admit. }
@@ -1114,9 +1023,7 @@ Proof.
         eapply is_ctrace_ub.
         rewrite list_lookup_insert // compile_tp_len -lookup_lt_is_Some //.
     * exists ctrace_ub.
-      split; first split.
-      { constructor. }
-      { done. }
+      split; first done.
       eapply is_ctrace_insert.
       { rewrite /compile_tp list_lookup_fmap enumerate_lookup' Htp //. }
       { rewrite /compile_expr_yield compile_expr_bind'; first done. admit. }
@@ -1134,20 +1041,18 @@ Lemma AllocN_free_locations n v σ ρs l efs :
   ∃ (l' : free_locations n σ), `l' = l.
 Proof. intros Hbase. by exists (to_free_location n v σ ρs l efs Hbase). Qed.
 
-Lemma step_in_thread e1 σ1 κs e2 σ2 efs tr tid tid' tp (k : val → itree heaplangE val) tx :
+Lemma step_in_thread e1 σ1 κs e2 σ2 efs tr tid tid' tp (k : val → itree heaplangE val) tx n :
   base_step e1 σ1 κs e2 σ2 efs →
   is_ctrace tr tid' (<[tid:=(v ← compile_expr_yield e2 ; k v)%itree]>tp
                     ++ compile_tp' efs) →
-  trace_invariant σ2 tx tr →
+  trace_invariant σ2 tx n tr →
   tp !! tid = Some (v ← compile_expr_yield e1 ; k v)%itree →
-  ∃ tr', trace_invariant σ1 tx tr' ∧ is_ctrace tr' tid tp.
+  ∃ tr', trace_invariant σ1 tx (S n) tr' ∧ is_ctrace tr' tid tp.
 Proof.
-  intros Hbase Htr (Hub&Hstinv) Htp.
+  intros Hbase Htr Hinv Htp.
   inversion Hbase; subst; simpl in Htr; rewrite ?app_nil_r in Htr.
   - exists (ctrace_step_yield tid' tr). repeat split.
-    { apply trace_invariant_postfix_postfix with (tr := tr); eauto.
-      repeat constructor. }
-    { by apply state_invariant_step_yield. }
+    { by apply trace_invariant_step_yield. }
     eapply is_ctrace_insert; first done.
     { rewrite /compile_expr_yield/compile_expr. eutt_norm/=. rewrite /step_ret. eutt_norm/=.
       reflexivity. }
@@ -1156,9 +1061,7 @@ Proof.
     rewrite list_insert_insert.
     by simpl_itree in Htr.
   - exists (ctrace_step_yield tid' tr). repeat split.
-    { apply trace_invariant_postfix_postfix with (tr := tr); eauto.
-      repeat constructor. }
-    { by apply state_invariant_step_yield. }
+    { by apply trace_invariant_step_yield. }
     eapply is_ctrace_insert; first done.
     { rewrite /compile_expr_yield/compile_expr. eutt_norm/=. rewrite /step_ret. eutt_norm/=.
       reflexivity. }
@@ -1167,9 +1070,7 @@ Proof.
     rewrite list_insert_insert.
     by simpl_itree in Htr.
   - exists (ctrace_step_yield tid' tr). repeat split.
-    { apply trace_invariant_postfix_postfix with (tr := tr); eauto.
-      repeat constructor. }
-    { by apply state_invariant_step_yield. }
+    { by apply trace_invariant_step_yield. }
     eapply is_ctrace_insert; first done.
     { rewrite /compile_expr_yield/compile_expr. eutt_norm/=. rewrite /step_ret. eutt_norm/=.
       reflexivity. }
@@ -1178,9 +1079,7 @@ Proof.
     rewrite list_insert_insert.
     by simpl_itree in Htr.
   - exists (ctrace_step_yield tid' tr). repeat split.
-    { apply trace_invariant_postfix_postfix with (tr := tr); eauto.
-      repeat constructor. }
-    { by apply state_invariant_step_yield. }
+    { by apply trace_invariant_step_yield. }
     eapply is_ctrace_insert; first done.
     { rewrite /compile_expr_yield/compile_expr. eutt_norm/=. rewrite /step_ret. eutt_norm/=.
       reflexivity. }
@@ -1189,104 +1088,79 @@ Proof.
     rewrite list_insert_insert.
     by simpl_itree in Htr.
   - pose (e' := subst' x v2 (subst' f (RecV f x e0) e0)).
+    exists (ctrace_step_yield tid' tr). repeat split.
+    { by apply trace_invariant_step_yield. }
     destruct (to_val e') as [v|] eqn:Hval.
-    * exists (CTYield tid' tr). repeat split.
-      { apply trace_invariant_postfix_postfix with (tr := tr); eauto.
-        repeat constructor. }
-      { by apply state_invariant_yield. }
-      eapply is_ctrace_insert; first done.
-      { rewrite /compile_expr_yield /= base_Beta /= /step_if_not_val /yield_if_not_val.
-        rewrite /e' in Hval. rewrite Hval. rewrite bind_ret_l.
+    * eapply is_ctrace_insert; first done.
+      { rewrite /compile_expr_yield /= base_Beta /= /yield_if_not_val.
+        rewrite /e' in Hval. rewrite Hval.
         eutt_norm/=. reflexivity. }
       rewrite /e' in Hval. apply of_to_val in Hval as Heq.
       rewrite -Heq in Htr. rewrite -Heq. rewrite /compile_expr. is_ctrace_norm/=. simpl_itree in Htr.
-      apply is_ctrace_yield with (t := k v).
+      apply is_ctrace_step_yield with (t := (k v)%itree).
       { rewrite list_lookup_insert //. by apply lookup_lt_is_Some. }
       by rewrite list_insert_insert.
-    * exists (ctrace_step_yield tid' tr). repeat split.
-      { apply trace_invariant_postfix_postfix with (tr := tr); eauto.
-        repeat constructor. }
-      { by apply state_invariant_step_yield. }
-      eapply is_ctrace_insert; first done.
-      { rewrite /compile_expr_yield /= base_Beta /= /yield_if_not_val /step_if_not_val.
+    * eapply is_ctrace_insert; first done.
+      { rewrite /compile_expr_yield /= base_Beta /= /yield_if_not_val.
         rewrite /e' in Hval. rewrite Hval. eutt_norm/=. reflexivity. }
-      rewrite /e' in Hval. rewrite /compile_expr_yield /yield_if_not_val /step_if_not_val in Htr.
+      rewrite /e' in Hval. rewrite /compile_expr_yield /yield_if_not_val in Htr.
       rewrite Hval in Htr.
       rewrite bind_bind in Htr. setoid_rewrite bind_bind in Htr. setoid_rewrite bind_ret_l in Htr.
       apply is_ctrace_step_yield with (t := (v ← compile_expr e'; yield ;; k v)%itree).
       { rewrite list_lookup_insert //. by apply lookup_lt_is_Some. }
       rewrite list_insert_insert //.
   - exists (ctrace_step_yield tid' tr). repeat split.
-    { apply trace_invariant_postfix_postfix with (tr := tr); eauto.
-      repeat constructor. }
-    { by apply state_invariant_step_yield. }
+    { by apply trace_invariant_step_yield. }
     rewrite /compile_expr_yield compile_expr_val !bind_ret_l in Htr.
     eapply is_ctrace_insert with (t' := (step ;; yield ;; k v')%itree); first done.
     { rewrite /compile_expr_yield base_UnOp //. eutt_norm/=. rewrite /step_ret. by eutt_norm/=. }
     eapply is_ctrace_step_yield. { rewrite list_lookup_insert //. by apply lookup_lt_is_Some. }
     by rewrite list_insert_insert.
   - exists (ctrace_step_yield tid' tr). repeat split.
-    { apply trace_invariant_postfix_postfix with (tr := tr); eauto.
-      repeat constructor. }
-    { by apply state_invariant_step_yield. }
+    { by apply trace_invariant_step_yield. }
     rewrite /compile_expr_yield compile_expr_val !bind_ret_l in Htr.
     eapply is_ctrace_insert with (t' := (step ;; yield ;; k v')%itree); first done.
     { rewrite /compile_expr_yield base_BinOp //. eutt_norm/=. rewrite /step_ret. by eutt_norm/=. }
     eapply is_ctrace_step_yield. { rewrite list_lookup_insert //. by apply lookup_lt_is_Some. }
     by rewrite list_insert_insert.
-  - destruct (to_val e2) eqn:Hval.
-    * exists (CTYield tid' tr). repeat split.
-      { apply trace_invariant_postfix_postfix with (tr := tr); eauto.
-        repeat constructor. }
-      { by apply state_invariant_yield. }
-      apply of_to_val in Hval as <-.
+  - exists (ctrace_step_yield tid' tr). repeat split.
+    { by apply trace_invariant_step_yield. }
+    destruct (to_val e2) eqn:Hval.
+    * apply of_to_val in Hval as <-.
       eapply is_ctrace_insert; first done.
       { rewrite /compile_expr_yield/compile_expr/=. eutt_norm/=. reflexivity. }
-      apply is_ctrace_yield with (t := k v).
+      apply is_ctrace_step_yield with (t := k v).
       { rewrite list_lookup_insert //. by apply lookup_lt_is_Some. }
       rewrite list_insert_insert.
       by simpl_itree in Htr.
-    * exists (ctrace_step_yield tid' tr). repeat split.
-      { apply trace_invariant_postfix_postfix with (tr := tr); eauto.
-        repeat constructor. }
-      { by apply state_invariant_step_yield. }
-      eapply is_ctrace_insert; first done.
+    * eapply is_ctrace_insert; first done.
       { rewrite /compile_expr_yield/compile_expr. eutt_norm/=.
-        rewrite /yield_if_not_val /step_if_not_val Hval /=. reflexivity. }
-      rewrite /compile_expr_yield/yield_if_not_val Hval in Htr. simpl_itree in Htr.
-      eapply is_ctrace_step_yield.
-      { rewrite list_lookup_insert //. by apply lookup_lt_is_Some. }
-      rewrite list_insert_insert.
-      by simpl_itree in Htr.
-  - destruct (to_val e2) eqn:Hval.
-    * exists (CTYield tid' tr). repeat split.
-      { apply trace_invariant_postfix_postfix with (tr := tr); eauto.
-        repeat constructor. }
-      { by apply state_invariant_yield. }
-      apply of_to_val in Hval as <-.
-      eapply is_ctrace_insert; first done.
-      { rewrite /compile_expr_yield/compile_expr. eutt_norm/=.
-        rewrite /step_if_not_val /=. reflexivity. }
-      apply is_ctrace_yield with (t := k v).
-      { rewrite list_lookup_insert //. by apply lookup_lt_is_Some. }
-      rewrite list_insert_insert.
-      by simpl_itree in Htr.
-    * exists (ctrace_step_yield tid' tr). repeat split.
-      { apply trace_invariant_postfix_postfix with (tr := tr); eauto.
-        repeat constructor. }
-      { by apply state_invariant_step_yield. }
-      eapply is_ctrace_insert; first done.
-      { simpl. rewrite /compile_expr_yield/compile_expr. eutt_norm/=.
-        rewrite /yield_if_not_val /step_if_not_val Hval /=. reflexivity. }
+        rewrite /yield_if_not_val Hval /=. reflexivity. }
       rewrite /compile_expr_yield/yield_if_not_val Hval in Htr. simpl_itree in Htr.
       eapply is_ctrace_step_yield.
       { rewrite list_lookup_insert //. by apply lookup_lt_is_Some. }
       rewrite list_insert_insert.
       by simpl_itree in Htr.
   - exists (ctrace_step_yield tid' tr). repeat split.
-    { apply trace_invariant_postfix_postfix with (tr := tr); eauto.
-      repeat constructor. }
-    { by apply state_invariant_step_yield. }
+    { by apply trace_invariant_step_yield. }
+    destruct (to_val e2) eqn:Hval.
+    * apply of_to_val in Hval as <-.
+      eapply is_ctrace_insert; first done.
+      { rewrite /compile_expr_yield/compile_expr. eutt_norm/=. reflexivity. }
+      apply is_ctrace_step_yield with (t := k v).
+      { rewrite list_lookup_insert //. by apply lookup_lt_is_Some. }
+      rewrite list_insert_insert.
+      by simpl_itree in Htr.
+    * eapply is_ctrace_insert; first done.
+      { simpl. rewrite /compile_expr_yield/compile_expr. eutt_norm/=.
+        rewrite /yield_if_not_val Hval /=. reflexivity. }
+      rewrite /compile_expr_yield/yield_if_not_val Hval in Htr. simpl_itree in Htr.
+      eapply is_ctrace_step_yield.
+      { rewrite list_lookup_insert //. by apply lookup_lt_is_Some. }
+      rewrite list_insert_insert.
+      by simpl_itree in Htr.
+  - exists (ctrace_step_yield tid' tr). repeat split.
+    { by apply trace_invariant_step_yield. }
     rewrite /compile_expr_yield compile_expr_val !bind_ret_l in Htr.
     eapply is_ctrace_insert with (t' := (step ;; yield ;; k v1)%itree); first done.
     { rewrite /compile_expr_yield/compile_expr. eutt_norm/=. rewrite /step_ret. eutt_norm/=.
@@ -1294,9 +1168,7 @@ Proof.
     eapply is_ctrace_step_yield. { rewrite list_lookup_insert //. by apply lookup_lt_is_Some. }
     by rewrite list_insert_insert.
   - exists (ctrace_step_yield tid' tr). repeat split.
-    { apply trace_invariant_postfix_postfix with (tr := tr); eauto.
-      repeat constructor. }
-    { by apply state_invariant_step_yield. }
+    { by apply trace_invariant_step_yield. }
     rewrite /compile_expr_yield compile_expr_val !bind_ret_l in Htr.
     eapply is_ctrace_insert with (t' := (step ;; yield ;; k v2)%itree); first done.
     { rewrite /compile_expr_yield/compile_expr. eutt_norm/=. rewrite /step_ret. eutt_norm/=.
@@ -1304,12 +1176,9 @@ Proof.
     eapply is_ctrace_step_yield. { rewrite list_lookup_insert //. by apply lookup_lt_is_Some. }
     by rewrite list_insert_insert.
   - exists (ctrace_step_yield tid' tr). repeat split.
-    { apply trace_invariant_postfix_postfix with (tr := tr); eauto.
-      repeat constructor. }
-    { by apply state_invariant_step_yield. }
+    { by apply trace_invariant_step_yield. }
     eapply is_ctrace_insert; first done.
-    { simpl. rewrite /compile_expr_yield/compile_expr. eutt_norm/=.
-      rewrite /step_if_not_val /=. reflexivity. }
+    { simpl. rewrite /compile_expr_yield/compile_expr. eutt_norm/=. reflexivity. }
     eapply is_ctrace_step_yield.
     { rewrite list_lookup_insert //. by apply lookup_lt_is_Some. }
     rewrite list_insert_insert.
@@ -1317,9 +1186,7 @@ Proof.
     setoid_rewrite bind_bind in Htr. setoid_rewrite bind_ret_l in Htr.
     by rewrite interp_recursive_call.
   - exists (ctrace_step_yield tid' tr). repeat split.
-    { apply trace_invariant_postfix_postfix with (tr := tr); eauto.
-      repeat constructor. }
-    { by apply state_invariant_step_yield. }
+    { by apply trace_invariant_step_yield. }
     eapply is_ctrace_insert; first done.
     { simpl. rewrite /compile_expr_yield/compile_expr. eutt_norm/=.
       rewrite /yield_if_not_val /=. reflexivity. }
@@ -1329,11 +1196,9 @@ Proof.
     setoid_rewrite bind_bind in Htr. setoid_rewrite bind_ret_l in Htr.
     by rewrite list_insert_insert interp_recursive_call.
   - destruct (AllocN_free_locations _ _ _ _ _ _ Hbase) as [ll <-].
-    exists (CTVis state (subevent _ EGetState) σ1 (CTVis (free_locations n σ1) (subevent _ (EDemonic (free_locations n σ1))) ll (CTVis () (subevent _ (ESetState (state_init_heap (`ll) n v σ1))) () (ctrace_step_yield tid' tr)))).
+    exists (CTVis state (subevent _ EGetState) σ1 (CTVis (free_locations n0 σ1) (subevent _ (EDemonic (free_locations n0 σ1))) ll (CTVis () (subevent _ (ESetState (state_init_heap (`ll) n0 v σ1))) () (ctrace_step_yield tid' tr)))).
     repeat split.
-    { apply trace_invariant_postfix_postfix with (tr := tr); eauto.
-      repeat constructor. }
-    { rewrite /trace_invariant_state /= decide_True //. by apply state_invariant_step_yield. }
+    { rewrite /= decide_True //. by apply trace_invariant_step_yield. }
     eapply is_ctrace_insert; first done.
     { simpl. rewrite /compile_expr_yield/compile_expr. eutt_norm/=. rewrite /step_ret. eutt_norm/=.
       reflexivity. }
@@ -1351,9 +1216,7 @@ Proof.
     rewrite list_insert_insert.
     by simpl_itree in Htr.
   - exists (ctrace_store' l None σ1 (ctrace_step_yield tid' tr)). repeat split.
-    { apply trace_invariant_postfix_postfix with (tr := tr); eauto.
-      repeat constructor. }
-    { rewrite /trace_invariant_state /= decide_True //. by apply state_invariant_step_yield. }
+    { rewrite /= decide_True //. by apply trace_invariant_step_yield. }
     eapply is_ctrace_insert; first done.
     { simpl. rewrite /compile_expr_yield/compile_expr. eutt_norm/=. rewrite /step_ret. eutt_norm/=.
       reflexivity. }
@@ -1364,9 +1227,7 @@ Proof.
     rewrite !list_insert_insert.
     by simpl_itree in Htr.
   - exists (ctrace_load σ2 (ctrace_step_yield tid' tr)). repeat split.
-    { apply trace_invariant_postfix_postfix with (tr := tr); eauto.
-      repeat constructor. }
-    { rewrite /trace_invariant_state /= decide_True //. by apply state_invariant_step_yield. }
+    { rewrite /= decide_True //. by apply trace_invariant_step_yield. }
     eapply is_ctrace_insert; first done.
     { simpl. rewrite /compile_expr_yield/compile_expr. eutt_norm/=. rewrite /step_ret. eutt_norm/=.
       reflexivity. }
@@ -1378,9 +1239,7 @@ Proof.
     rewrite list_insert_insert.
     by simpl_itree in Htr.
   - exists (ctrace_store l w σ1 (ctrace_step_yield tid' tr)). repeat split.
-    { apply trace_invariant_postfix_postfix with (tr := tr); eauto.
-      repeat constructor. }
-    { rewrite /trace_invariant_state /= decide_True //. by apply state_invariant_step_yield. }
+    { rewrite /= decide_True //. by apply trace_invariant_step_yield. }
     eapply is_ctrace_insert; first done.
     { simpl. rewrite /compile_expr_yield/compile_expr. eutt_norm/=. rewrite /step_ret. eutt_norm/=.
       reflexivity. }
@@ -1392,9 +1251,7 @@ Proof.
     rewrite list_insert_insert.
     by simpl_itree in Htr.
   - exists (ctrace_store l v2 σ1 (ctrace_step_yield tid' tr)). repeat split.
-    { apply trace_invariant_postfix_postfix with (tr := tr); eauto.
-      repeat constructor. }
-    { rewrite /trace_invariant_state /= decide_True //. by apply state_invariant_step_yield. }
+    { rewrite /= decide_True //. by apply trace_invariant_step_yield. }
     eapply is_ctrace_insert; first done.
     { simpl. rewrite /compile_expr_yield/compile_expr. eutt_norm/=. rewrite /step_ret. eutt_norm/=.
       reflexivity. }
@@ -1406,13 +1263,10 @@ Proof.
     rewrite list_insert_insert.
     by simpl_itree in Htr.
   - destruct (decide (vl = v1)) as [->|Hneq].
-    * rewrite bool_decide_eq_true_2 // in Hstinv.
-      rewrite bool_decide_eq_true_2 // in Hbase.
+    * rewrite bool_decide_eq_true_2 // in Hinv.
       rewrite bool_decide_eq_true_2 // in Htr.
       exists (ctrace_load σ1 (ctrace_store l v2 σ1 (ctrace_step_yield tid' tr))). repeat split.
-      { apply trace_invariant_postfix_postfix with (tr := tr); eauto.
-        repeat constructor. }
-      { rewrite /trace_invariant_state /= !decide_True //. by apply state_invariant_step_yield. }
+      { rewrite /= !decide_True //. by apply trace_invariant_step_yield. }
       eapply is_ctrace_insert; first done.
       { simpl. rewrite /compile_expr_yield/compile_expr. eutt_norm/=. reflexivity. }
       eapply is_ctrace_load; first done.
@@ -1426,13 +1280,10 @@ Proof.
       { rewrite list_lookup_insert //. by apply lookup_lt_is_Some. }
       rewrite list_insert_insert.
       by simpl_itree in Htr.
-    * rewrite bool_decide_eq_false_2 // in Hstinv.
-      rewrite bool_decide_eq_false_2 // in Hbase.
+    * rewrite bool_decide_eq_false_2 // in Hinv.
       rewrite bool_decide_eq_false_2 // in Htr.
       exists (ctrace_load σ1 (ctrace_step_yield tid' tr)). repeat split.
-      { apply trace_invariant_postfix_postfix with (tr := tr); eauto.
-        repeat constructor. }
-      { rewrite /trace_invariant_state /= !decide_True //. by apply state_invariant_step_yield. }
+      { rewrite /= !decide_True //. by apply trace_invariant_step_yield. }
       eapply is_ctrace_insert; first done.
       { simpl. rewrite /compile_expr_yield/compile_expr. eutt_norm/=. reflexivity. }
       eapply is_ctrace_load; first done.
@@ -1443,9 +1294,7 @@ Proof.
       rewrite list_insert_insert.
       by simpl_itree in Htr.
   - exists (ctrace_load σ1 (ctrace_store l (LitV (LitInt (i1 + i2))) σ1 (ctrace_step_yield tid' tr))). repeat split.
-    { apply trace_invariant_postfix_postfix with (tr := tr); eauto.
-      repeat constructor. }
-    { rewrite /trace_invariant_state /= !decide_True //. by apply state_invariant_step_yield. }
+    { rewrite /= !decide_True //. by apply trace_invariant_step_yield. }
     eapply is_ctrace_insert; first done.
     { simpl. rewrite /compile_expr_yield/compile_expr. eutt_norm/=. reflexivity. }
     eapply is_ctrace_load; first done.
@@ -1460,9 +1309,7 @@ Proof.
     by simpl_itree in Htr.
   - exists (CTFork (compile_expr_kill e) (ctrace_step_yield tid' tr)).
     repeat split.
-    { apply trace_invariant_postfix_postfix with (tr := tr); eauto.
-      repeat constructor. }
-    { by apply state_invariant_step_yield. }
+    { by apply trace_invariant_step_yield. }
     rewrite /compile_expr_yield compile_expr_val !bind_ret_l in Htr.
     eapply is_ctrace_insert; first done.
     { simpl. rewrite /compile_expr_yield. eutt_norm/=. reflexivity. }
@@ -1487,16 +1334,16 @@ Lemma has_trace n tp σ tp' σ' κ tx :
   tp_termination tp' σ' tx →
   length tp > 0 →
   ∃ tid tr,
-    trace_invariant σ tx tr ∧
+    trace_invariant σ tx n tr ∧
     is_ctrace (R := val) tr tid (compile_tp tp).
 Proof.
   revert tp σ tp' σ' κ. induction n as [|n IH]; intros tp σ tp' σ' κ Hstep Hterm Hne.
   { destruct tx as [r|].
     - assert (Hterm' := Hterm).
       apply is_ctrace_ret  in Hterm as Htr.
-      apply trace_invariant_ret with (σ := σ') in Hterm' as Htinv.
+      apply trace_invariant_ret with (σ := σ') (n := 0) in Hterm' as Htinv.
       exists 0, (CTRet r). inversion Hstep. subst. by split.
-    - inversion Hstep; subst.
+    - inversion Hstep; subst. destruct u.
       apply stuck_ub in Hterm as (tid&tr&Hinv&Htr); eauto.
   }
   inversion Hstep as [|m [tp1 σ1] [tp2 σ2] [tp3 σ3] ? ? Hstep'' Hstep']. subst.
@@ -1515,12 +1362,12 @@ Proof.
     }
     destruct (decide (length tpa = 0)) as [Htpa|Htpa].
     * apply nil_length_inv in Htpa as ->. simpl. simpl in *.
-      apply step_in_thread with (tp := ((v ← compile_expr_yield e1 ; Ret v)%itree :: compile_tp' tpb)) (tid := 0) (tid' := tid) (k := λ v, Ret v) (tr := tr) (tx := tx) in Hbase as [tr' [Hinv' Htr']].
+      apply step_in_thread with (tp := ((v ← compile_expr_yield e1 ; Ret v)%itree :: compile_tp' tpb)) (tid := 0) (tid' := tid) (k := λ v, Ret v) (tr := tr) (tx := tx) (n := n) in Hbase as [tr' [Hinv' Htr']].
       + exists 0, tr'. rewrite compile_tp_cons //.
       + simpl. rewrite compile_tp_cons compile_tp'_app // in Htr.
       + done.
       + done.
-    * apply step_in_thread with (tp := (compile_tp tpa ++ (compile_expr_kill e1)%itree :: compile_tp' tpb)) (tid := length (compile_tp tpa)) (tid' := tid) (k := λ v, kill_thread) (tr := tr) (tx := tx) in Hbase as [tr' [Hinv' Htr']].
+    * apply step_in_thread with (tp := (compile_tp tpa ++ (compile_expr_kill e1)%itree :: compile_tp' tpb)) (tid := length (compile_tp tpa)) (tid' := tid) (k := λ v, kill_thread) (tr := tr) (tx := tx) (n := n) in Hbase as [tr' [Hinv' Htr']].
       + exists (length (compile_tp tpa)), tr'. rewrite compile_tp_app //.
       + replace (length (compile_tp tpa)) with (length (compile_tp tpa) + 0) by lia.
         rewrite compile_tp_app // in Htr.
@@ -1534,7 +1381,7 @@ Proof.
     }
     destruct (decide (length tpa = 0)) as [Htpa|Htpa].
     * apply nil_length_inv in Htpa as ->. simpl. simpl in *.
-      apply step_in_thread with (tp := ((v ← compile_expr_yield e1; w ← compile_expr (fill K (Val v)); yield ;; Ret w)%itree :: compile_tp' tpb)) (tid := 0) (tid' := tid) (k := λ v, (w ← compile_expr (fill K (Val v)); yield ;; Ret w)%itree) (tr := tr) (tx := tx) in Hbase as [tr' [Hinv' Htr']].
+      apply step_in_thread with (tp := ((v ← compile_expr_yield e1; w ← compile_expr (fill K (Val v)); yield ;; Ret w)%itree :: compile_tp' tpb)) (tid := 0) (tid' := tid) (k := λ v, (w ← compile_expr (fill K (Val v)); yield ;; Ret w)%itree) (tr := tr) (tx := tx) (n := n) in Hbase as [tr' [Hinv' Htr']].
       + exists 0, tr'.
         split; first done.
         rewrite compile_tp_cons /= /compile_expr_yield compile_expr_bind.
@@ -1554,7 +1401,7 @@ Proof.
       + done.
     * rewrite compile_tp_app // in Htr.
       rewrite compile_tp_app //.
-      apply step_in_thread with (tp := (compile_tp tpa ++ (v ← compile_expr e1; yield_if_not_val e1;; compile_expr_kill (fill K (Val v)))%itree :: compile_tp' tpb)) (tid := length tpa) (tid' := tid) (k := λ v, (compile_expr (fill K (Val v));; yield ;; kill_thread)%itree) (tr := tr) (tx := tx) in Hbase as [tr' [Hinv' Htr']].
+      apply step_in_thread with (tp := (compile_tp tpa ++ (v ← compile_expr e1; yield_if_not_val e1;; compile_expr_kill (fill K (Val v)))%itree :: compile_tp' tpb)) (tid := length tpa) (tid' := tid) (k := λ v, (compile_expr (fill K (Val v));; yield ;; kill_thread)%itree) (tr := tr) (tx := tx) (n := n) in Hbase as [tr' [Hinv' Htr']].
       + exists (length tpa), tr'.
         split; first done.
         rewrite /= /compile_expr_kill/compile_expr_yield compile_expr_bind.
@@ -1574,325 +1421,105 @@ Proof.
       + done.
 Admitted.
 
-Lemma interp_tr_state_ub {E R S} `{EqDecision S} `{ubE -< E} σ (tr : trace (stateE S +' E) R) tr' :
-  trace_terminates_in tr TermUb →
-  interp_tr_state σ tr = Some tr' →
-  trace_terminates_in tr' TermUb.
-Proof.
-  revert σ tr'. induction tr; intros σ tr' Hub Hst.
-  - inversion Hub.
-  - destruct e as [e|e]; first destruct e as [|σ'].
-    * simpl in Hst. destruct (decide (a = σ)) as [->|]; last discriminate.
-      apply IHtr with (σ := σ); last done. by inversion Hub.
-    * inversion Hub; simplify_K; simplify_K; subst. by eapply IHtr.
-    * simpl in Hst. destruct (interp_tr_state σ tr) as [tr''|] eqn:Heq.
-      + simpl in Heq. injection Hst as <-. constructor.
-        by apply IHtr with (σ := σ); first by inversion Hub.
-      + discriminate.
-  - inversion Hub; simplify_K; simplify_K; subst.
-    injection Hst as <-. simplify_K. constructor.
-  - inversion Hub.
-Qed.
-
-Lemma interp_tr_term {E E' R} `{ubE -< E'} (tr : trace (E +' E') R) (tx : Terminal R) :
-  trace_terminates_in tr tx →
-  trace_terminates_in (interp_tr tr) tx.
-Proof.
-  intros Hterm.
-  induction tr.
-  - rewrite /= /trace_terminates_in. rewrite /trace_terminates_in in Hterm.
-    destruct tx; inversion Hterm. subst. constructor.
-  - simpl. destruct e.
-    * apply IHtr. destruct tx; inversion Hterm; by simplify_K.
-    * constructor. apply IHtr. destruct tx; inversion Hterm; by simplify_K.
-  - rewrite /= /trace_terminates_in. rewrite /trace_terminates_in in Hterm.
-    destruct tx; inversion Hterm. subst. constructor.
-  - rewrite /= /trace_terminates_in. rewrite /trace_terminates_in in Hterm.
-    destruct tx; inversion Hterm.
-Qed.
-
-Lemma sequencify_term {E E' R} `{ubE -< E'} (tr : ctrace (E +' E') R) (tx : Terminal R) :
-  ctrace_terminates_in tr tx →
-  trace_terminates_in (sequencify tr) (inl <$> tx).
-Proof.
-  intros Hterm.
-  induction tr.
-  - rewrite /= /trace_terminates_in. rewrite /trace_terminates_in in Hterm.
-    destruct tx; inversion Hterm. subst. constructor.
-  - simpl. constructor. apply IHtr. destruct tx; inversion Hterm; by simplify_K.
-  - rewrite /= /trace_terminates_in.
-    destruct tx; inversion Hterm. subst. constructor.
-  - simpl. apply IHtr. destruct tx; inversion Hterm; by simplify_K.
-  - simpl. apply IHtr. destruct tx; inversion Hterm; by simplify_K.
-  - rewrite /= /trace_terminates_in. destruct tx; inversion Hterm.
-  - simpl. apply IHtr. destruct tx; inversion Hterm; by simplify_K.
-  - rewrite /= /trace_terminates_in. destruct tx; inversion Hterm.
-Qed.
-
-Lemma interp_tr_state_ret {E R S} `{EqDecision S} `{ubE -< E} σ (tr : trace (stateE S +' E) R) tr' (r : R) :
-  trace_terminates_in tr (TermRet r) →
-  interp_tr_state σ tr = Some tr' →
-  ∃ σ, trace_terminates_in tr' (TermRet (σ, r)).
-Proof.
-  revert σ tr'. induction tr; intros σ tr' Hret Hst.
-  - inversion Hret. injection Hst as <-. exists σ. constructor.
-  - destruct e as [e|e]; first destruct e as [|σ'].
-    * simpl in Hst. destruct (decide (a = σ)) as [->|]; last discriminate.
-      apply IHtr with (σ := σ); last done. by inversion Hret.
-    * inversion Hret; simplify_K; simplify_K; subst. by eapply IHtr.
-    * simpl in Hst. destruct (interp_tr_state σ tr) as [tr''|] eqn:Heq.
-      + simpl in Heq. injection Hst as <-.
-        inversion Hret. subst. simplify_K.
-        apply IHtr in Heq as [σ' Hterm]; last done.
-        exists σ'. by constructor.
-      + discriminate.
-  - inversion Hret; simplify_K; simplify_K; subst.
-  - inversion Hret.
-Qed.
-
-Inductive terminates_in' {R} : itree' (laterE +' ubE) R → Terminal R → Prop :=
-  | terminates_in_ELater tx k :
-  terminates_in' (observe (k ())) tx →
-  terminates_in' (VisF (inl1 ELater) k) tx
-  | terminates_in_Tau tx t :
-  terminates_in' (observe t) tx →
-  terminates_in' (TauF t) tx
-  | terminates_in_EUb k :
-  terminates_in' (VisF (inr1 EUb) k) TermUb
-  | terminates_in_Ret r :
-  terminates_in' (RetF r) (TermRet r).
-Definition terminates_in {R} (t : itree (laterE +' ubE) R) (tx : Terminal R) : Prop :=
-  terminates_in' (observe t) tx.
-Fixpoint model_terminal {R} (laters : nat) (tx : Terminal R) : itree (laterE +' ubE) R :=
-  match laters with
-  | O =>
-    match tx with
-    | TermRet r => Ret r
-    | TermUb => ub
-    end
-  | S n => step ;; model_terminal n tx
-  end.
-Lemma terminates_in_model {R} (t : itree (laterE +' ubE) R) tx :
-  terminates_in t tx →
-  ∃ n, t ≈ model_terminal n tx.
-Proof.
-  intros Hterm. rewrite /terminates_in in Hterm.
-  remember (observe t) as ot. revert t Heqot. induction Hterm; intros t' Heqot.
-  - destruct (IHHterm (k ())) as [n Heutt]; first done.
-    exists (S n). simplify_obs. simpl. rewrite bind_trigger.
-    f_equiv. f_equiv. by intros [].
-  - destruct (IHHterm t) as [n Heutt]; first done.
-    exists n. simplify_obs. by transitivity t; first by apply tau_eutt.
-  - exists 0. simplify_obs. simpl. rewrite /ub. f_equiv. f_equiv. intros [].
-  - exists 0. by simplify_obs.
-Qed.
-
-Lemma is_trace_term {R} (t : itree (laterE +' ubE) R) tr tx :
-  trace_terminates_in tr tx →
-  is_trace tr t →
-  terminates_in t tx.
-Proof.
-  intros Hterm Htr. rewrite /terminates_in. induction Htr.
-  - destruct tx; inversion Hterm. by constructor.
-  - destruct e as [e|e]; destruct e, a.
-    constructor. apply IHHtr. destruct tx; by inversion Hterm.
-  - destruct tx; inversion Hterm. destruct e as [e|e]; first by destruct e.
-    destruct e. constructor.
-  - destruct tx; inversion Hterm.
-  - constructor. by apply IHHtr.
-Qed.
-
 Lemma execution n e σ tp' σ' κ tx :
   language.nsteps n ([e], σ) κ (tp', σ') →
   tp_termination tp' σ' tx →
-  ∃ t1 t2 t3,
-    (* TODO: consisting naming for interpretion relations *)
-    (* TODO: abstraction for this composite relation *)
-    threadpool_irel (R := val) (compile_expr_yield e) t1 ∧
-    demonic_irel t1 t2 ∧
-    state_irel σ t2 t3 ∧
-    (* TODO: use UB adequacy *)
+  ∃ te,
+    heaplang_eval e σ (Some n) te ∧
     match tx with
-    | TermUb => terminates_in t3 TermUb
-    | TermRet r => ∃ σ', terminates_in t3 (TermRet (σ', inl r))
+    | TermUb => te ≈ Ret (inr UbCrash)
+    | TermRet r => ∃ σ', te ≈ Ret (inl (inl (σ', inl r)))
     end.
 Proof.
   intros Hsteps Hterm.
-  apply has_trace with (tx := tx) in Hsteps as (tid&tr&[Htinv Hstinv]&Htr); eauto.
-  rewrite /trace_invariant_state in Hstinv.
+  apply has_trace with (tx := tx) in Hsteps as (tid&tr&Hinv&Htr); eauto.
+  rewrite /trace_invariant in Hinv.
   destruct (interp_tr_state σ (interp_tr (sequencify tr))) as [tr'|] eqn:Heq;
-    rewrite Heq // in Hstinv.
-  rewrite /trace_invariant_postfix in Htinv.
+    rewrite Heq // in Hinv.
   apply threadpool_trace in Htr as (t1&Hint&Htr).
-  exists t1.
   eapply demonic_trace in Htr as (t2&Hinst&Htr).
-  exists t2.
   eapply state_trace with (s := σ) in Htr as (t3&Heval&Htr); last done.
-  exists t3.
+  eapply later_trace with (n := Some n) in Htr.
+  eapply void_trace in Htr.
+  eapply ub_trace in Htr.
+  exists (ub_ifn (insert_voidE (later_ifn (Some n) t3))).
   split.
-  { destruct (interleaves_lookup _ _ _ Hint) as [t Hidx].
-    destruct tid; last discriminate.
-    rewrite /compile_tp in Hint. simpl in Hint.
-    rewrite (bisimulation_is_eq _ _ (bind_ret_r (compile_expr_yield e))) in Hint.
-    apply Hint.
-  }
-  split; first done.
-  split; first done.
-  destruct tx.
-  - apply sequencify_term in Htinv. apply interp_tr_term in Htinv.
-    eapply interp_tr_state_ret in Htinv as [σ'' Htinv]; last done.
-    exists σ''. by apply is_trace_term with (t := t3) (tr := tr') (tx := TermRet (σ'', inl r)).
-  - apply is_trace_term with (t := t3) (tr := tr') (tx := TermUb); eauto.
-    eapply interp_tr_state_ub; last done. apply interp_tr_term. by apply sequencify_term in Htinv.
-Qed.
-
-Lemma model_wpi {R} `{!invGS_gen hlc Σ} M n (tx : Terminal R) (Φ : R → iProp Σ) :
-  WPi (model_terminal n tx) @ laterH Identity ⊕ ubH ; M {{ Φ }} -∗
-  |={M}=> match tx with
-  | TermUb => False
-  | TermRet v => Φ v
-  end.
-Proof.
-  induction n; iIntros "Hwp".
-  - simpl. destruct tx.
-    * rewrite -wpi_ret' //.
-    * by iDestruct (wpi_ub with "Hwp") as "Hwp".
-  - iApply IHn. rewrite /= bind_vis -wpi_vis' /= wpi_clear_mask. by simpl_itree.
-Qed.
-
-Lemma model_wpi_later' {R} `{!invGS_gen hlc Σ} n (tx : Terminal R) (Φ : R → iProp Σ) :
-  WPi (model_terminal n tx) @ laterH Later ⊕ ubH ; ∅ {{ Φ }} -∗
-  |={∅}=> |={∅}▷=>^n match tx with
-  | TermUb => False
-  | TermRet v => Φ v
-  end.
-Proof.
-  induction n; iIntros "Hwp".
-  - simpl. destruct tx.
-    * rewrite -wpi_ret' //.
-    * by iDestruct (wpi_ub with "Hwp") as "Hwp".
-  - iModIntro. simpl. iApply IHn. rewrite /= bind_vis -wpi_vis' /=.
-    iMod "Hwp". iModIntro. iNext.
-    simpl_itree. iApply wpi_clear_mask. by iModIntro.
-Qed.
-
-Lemma model_wpi_later {R} `{!invGS_gen hlc Σ} M n (tx : Terminal R) (Φ : R → iProp Σ) :
-  WPi (model_terminal n tx) @ laterH Later ⊕ ubH ; M {{ Φ }} -∗
-  |={M, ∅}=> |={∅}▷=>^n match tx with
-  | TermUb => False
-  | TermRet v => |={∅, M}=> Φ v
-  end.
-Proof.
-  iIntros "Hwp".
-  iDestruct (wpi_clear_mask with "Hwp") as "Hwp".
-  iDestruct (model_wpi_later' with "Hwp") as "Hpost".
-  by iMod "Hpost".
+  - exists t1, t2, t3.
+    split.
+    { destruct (interleaves_lookup _ _ _ Hint) as [t Hidx].
+      destruct tid; last discriminate.
+      rewrite /compile_tp in Hint. simpl in Hint.
+      rewrite (bisimulation_is_eq _ _ (bind_ret_r (compile_expr_yield e))) in Hint.
+      apply Hint.
+    }
+    split; first done.
+    split; first done.
+    done.
+  - destruct tx.
+    * rewrite /tr_terminal in Hinv.
+      destruct (interp_tr_ub (insert_voidE_tr (interp_tr_later (Some n) tr'))) as [[[[σ_ [r|]]|]|] | | | ] eqn:Heq';
+        rewrite Heq' in Hinv; try contradiction.
+      exists σ_.
+      apply void_trace_ret_inv in Htr as ->. by apply bool_decide_unpack in Hinv as ->.
+    * destruct u.
+      destruct (interp_tr_ub (insert_voidE_tr (interp_tr_later (Some n) tr'))) as [[[[σ_ [r|]]|]|] | | | ] eqn:Heq';
+        rewrite Heq' in Hinv; try contradiction.
+      apply void_trace_ret_inv in Htr as ->. by destruct u.
 Qed.
 
 End adequacy.
 
-Lemma execution_wpi' n e σ tp' σ' κ tx:
+(* TODO: Don't redefine *)
+Notation TermUb := (inr UbCrash).
+Notation TermRet r := (inl r).
+
+Lemma execution_wpi Σ (Hinv : invGS_gen HasLc Σ) (Hhl : heaplangHGS Σ) Φ n e σ tp' σ' κ tx:
   language.nsteps n ([e], σ) κ (tp', σ') →
   tp_termination tp' σ' tx →
-  (∀ hlc Σ (Hinv : invGS_gen hlc Σ) (Hhl : heaplangHGS Σ) Φ,
-      state_interp σ -∗
-  WPi (compile_expr_yield e) @ heaplangH Identity ; ⊤ {{ Φ }} -∗
+  state_interp σ -∗
+  heap_inv -∗
+  WP e @ Identity ; ⊤ {{ Φ }} -∗
   |={⊤}=> match tx with
   | TermUb => False
   | TermRet v => Φ v
-  end).
-Proof.
-  iIntros (Hstep Hstuck ? ? ? ? ?).
-  apply execution with (tx := tx) in Hstep as (t1&t2&t3&Hint&Hinst&Heval&Hterm); last done.
-  iIntros "Hstate Hwp".
-  (* TODO: Name these adequacy theorems consistently. *)
-  iDestruct (threadpool_adequacy with "Hwp") as "Hwp"; first apply Hint.
-  iDestruct (demonic_adequacy with "Hwp") as "Hwp"; first apply Hinst.
-  iDestruct (state_adequacy with "Hstate Hwp") as "Hwp"; first apply Heval.
-  destruct tx.
-  - destruct Hterm as [σ'' [n' ->]%terminates_in_model].
-    iDestruct (model_wpi with "Hwp") as "Hwp".
-    by iMod "Hwp" as "[_ HΦ]".
-  - apply terminates_in_model in Hterm as [n' ->].
-    by iDestruct (model_wpi with "Hwp") as "Hwp".
-Qed.
-
-Lemma execution_wpi_later' n e σ tp' σ' κ tx :
-  language.nsteps n ([e], σ) κ (tp', σ') →
-  tp_termination tp' σ' tx →
-  ∃ n,
-    (∀ hlc Σ (Hinv : invGS_gen hlc Σ) (Hhl : heaplangHGS Σ) Φ,
-    state_interp σ -∗
-    WPi (compile_expr_yield e) @ heaplangH Later ; ⊤ {{ Φ }} -∗
-    |={⊤, ∅}=> |={∅}▷=>^n match tx with
-    | TermUb => False
-    | TermRet v => |={∅, ⊤}=> Φ v
-    end).
+  end.
 Proof.
   iIntros (Hstep Hstuck).
-  apply execution with (tx := tx) in Hstep as (t1&t2&t3&Hint&Hinst&Heval&Hterm); last done.
+  apply execution with (tx := tx) in Hstep as (te&Heval&Hterm); last done.
+  iIntros "Hstate #Hinv Hwp".
+  iDestruct (heaplang_adequacy_eval with "[] Hstate Hinv Hwp") as "HΦ".
+  { done. }
+  { iIntros ([=]). }
   destruct tx.
-  - destruct Hterm as [σ'' [n' Ht3]%terminates_in_model].
-    exists n'.
-    iIntros (? ? ? ? ?) "Hstate Hwp".
-    (* TODO: Name these adequacy theorems consistently. *)
-    iDestruct (threadpool_adequacy with "Hwp") as "Hwp"; first apply Hint.
-    iDestruct (demonic_adequacy with "Hwp") as "Hwp"; first apply Hinst.
-    iDestruct (state_adequacy with "Hstate Hwp") as "Hwp"; first apply Heval.
-    rewrite Ht3.
-    iDestruct (model_wpi_later with "Hwp") as "Hwp".
-    iMod "Hwp". iModIntro.
-    iApply step_fupdN_mono; last done. iIntros "[_ $]".
-  - apply terminates_in_model in Hterm as [n' Ht3].
-    exists n'.
-    iIntros (? ? ? ? ?) "Hstate Hwp".
-    (* TODO: Name these adequacy theorems consistently. *)
-    iDestruct (threadpool_adequacy with "Hwp") as "Hwp"; first apply Hint.
-    iDestruct (demonic_adequacy with "Hwp") as "Hwp"; first apply Hinst.
-    iDestruct (state_adequacy with "Hstate Hwp") as "Hwp"; first apply Heval.
-    rewrite Ht3.
-    iDestruct (model_wpi_later with "Hwp") as "Hwp".
-    iMod "Hwp". iModIntro.
-    iApply step_fupdN_mono; last done. iIntros "$".
+  - iMod "HΦ" as "[%r [%Heutt HΦ]]". destruct Hterm as [σ_ Heutt'].
+    rewrite Heutt in Heutt'. apply eqit_inv_Ret in Heutt' as ->.
+    by iMod "HΦ" as "[_ $]".
+  - iMod "HΦ" as "[%r [%Heutt HΦ]]". destruct u.
+    rewrite Heutt in Hterm. by apply eqit_inv_Ret in Hterm as ->.
 Qed.
 
-Lemma compile_expr_execution_wpi' n e σ tp' σ' κ tx :
+Lemma execution_wpi_later Σ (Hinv : invGS_gen HasLc Σ) (Hhl : heaplangHGS Σ) Φ n e σ tp' σ' κ tx :
   language.nsteps n ([e], σ) κ (tp', σ') →
   tp_termination tp' σ' tx →
-  (∀ hlc Σ (Hinv : invGS_gen hlc Σ) (Hhl : heaplangHGS Σ) Φ,
+  £ n -∗
   state_interp σ -∗
-  WPi (compile_expr e) @ heaplangH Identity ; ⊤ {{ Φ }} -∗
-  |={⊤}=> match tx with
-  | TermUb => False
-  | TermRet v => Φ v
-  end).
-Proof.
-  iIntros (Hstep Hterm ? ? ? ? ?) "Hstate Hwp".
-  iApply (execution_wpi' with "Hstate"); eauto.
-  iApply wpi_bind. iApply wpi_wand; last done.
-  iIntros (r) "HΦ". iApply wpi_bind. rewrite /yield_if_not_val. destruct (to_val _).
-  - iApply wpi_ret. by iApply wpi_ret.
-  - iApply @wpi_yield. by iApply wpi_ret.
-Qed.
-
-Lemma compile_expr_execution_wpi_later n e σ tp' σ' κ tx :
-  language.nsteps n ([e], σ) κ (tp', σ') →
-  tp_termination tp' σ' tx →
-  ∃ n,
-  (∀ hlc Σ (Hinv : invGS_gen hlc Σ) (Hhl : heaplangHGS Σ) Φ,
-  state_interp σ -∗
-  WPi (compile_expr e) @ heaplangH Later ; ⊤ {{ Φ }} -∗
-  |={⊤, ∅}=> |={∅}▷=>^n match tx with
+  heap_inv -∗
+  WP e @ Later ; ⊤ {{ Φ }} -∗
+  |={⊤, ∅}=> match tx with
   | TermUb => False
   | TermRet v => |={∅, ⊤}=> Φ v
-  end).
+  end.
 Proof.
-  iIntros (Hstep Hterm).
-  odestruct (execution_wpi_later' _ _ _ _ _ _ _ _ _) as [n' Hwp]; eauto.
-  exists n'. iIntros (? ? ? ? ?) "Hstate Hwp". iApply (Hwp with "Hstate").
-  iApply wpi_bind. iApply wpi_wand; last done.
-  iIntros (r) "HΦ". iApply wpi_bind. iApply wpi_yield_if_not_val.
-  by iApply wpi_ret.
+  iIntros (Hstep Hstuck).
+  apply execution with (tx := tx) in Hstep as (te&Heval&Hterm); last done.
+  iIntros "Hlc Hstate #Hinv Hwp".
+  iDestruct (heaplang_adequacy_eval with "[Hlc] Hstate Hinv Hwp") as "HΦ"; eauto.
+  destruct tx.
+  - iMod "HΦ" as "[%r [%Heutt HΦ]]". destruct Hterm as [σ_ Heutt'].
+    rewrite Heutt in Heutt'. apply eqit_inv_Ret in Heutt' as ->.
+    iModIntro. by iMod "HΦ" as "[_ $]".
+  - iMod "HΦ" as "[%r [%Heutt HΦ]]". destruct u.
+    rewrite Heutt in Hterm. by apply eqit_inv_Ret in Hterm as ->.
 Qed.
 
 From iris.program_logic Require Import adequacy.
@@ -1904,26 +1531,24 @@ Theorem heap_adequacy_later Σ `{!invGpreS Σ} `{!heaplangHGpreS Σ} e σ φ:
 Proof.
   move => Hwp. apply adequate_alt => t2 σ2 /erased_steps_nsteps[n [κs Hsteps]].
   constructor.
-  - move => ? ? ?.
-    odestruct (compile_expr_execution_wpi_later _) as [n' Had]; [done| |].
-    { subst. by constructor. }
-    apply: (heaplang_soundness n').
-    iIntros (? ?) "Hinv ??". iMod (Had with "[$] [Hinv]") as "Had".
-    { iPoseProof Hwp as "Hwp". rewrite wp_heaplang_eq. by iApply "Hwp". }
+  - move => ? ? Hval.
+    apply: (heaplang_soundness n). intros ? ?.
+    iDestruct (Hwp _ _) as "Hwp".
+    opose proof (execution_wpi_later _ _ _) as Had.
+    iIntros "Hinv Hs Hlc". iMod (Had with "Hlc Hs Hinv Hwp") as "Had"; eauto.
+    { rewrite Hval. apply tp_termination_TermRet. }
     (* TODO: find a less hacky way to do this *)
-    destruct n'.
-    + simpl. iMod "Had". iApply fupd_mask_intro; [done|]. by iIntros "?".
-    + iModIntro. iApply step_fupdN_S_fupd. iApply (step_fupdN_wand with "Had").
-      iIntros ">$". iApply fupd_mask_intro; [done|]. by iIntros "?".
+    simpl. iMod "Had". iApply fupd_mask_intro; first done. iIntros "_".
+    by iApply step_fupdN_intro.
   - move => e2 _ /elem_of_list_lookup [? He2].
     destruct (decide (not_stuck e2 σ2)) as [?| Hstuck%not_not_stuck]; [done|].
     exfalso.
-    odestruct (compile_expr_execution_wpi_later _) as [n' Had]; [done| |].
-    { apply tp_termination_TermUb. eexists _, _. done. }
-    apply: (heaplang_soundness n').
-    iIntros (? ?) "Hinv ??". iMod (Had with "[$] [Hinv]") as "Had".
-    { iPoseProof Hwp as "Hwp". rewrite wp_heaplang_eq. by iApply "Hwp". }
-    iModIntro. iApply (step_fupdN_wand with "Had"). by iIntros (?).
+    apply: (heaplang_soundness n). intros ? ?.
+    iDestruct (Hwp _ _) as "Hwp".
+    opose proof (execution_wpi_later _ _ _) as Had.
+    iIntros "Hinv Hs Hlc". iMod (Had with "Hlc Hs Hinv Hwp") as "Had"; eauto.
+    { apply tp_termination_TermUb. econstructor. by eexists. }
+    done.
 Qed.
 
 (* TODO: prove this via weakening *)
@@ -1933,20 +1558,22 @@ Theorem heap_adequacy_no_later Σ `{!invGpreS Σ} `{!heaplangHGpreS Σ} e σ φ:
 Proof.
   move => Hwp. apply adequate_alt => t2 σ2 /erased_steps_nsteps[n [κs Hsteps]].
   constructor.
-  - move => ? ? ?.
-    apply: (heaplang_soundness 0).
-    iIntros (? ?) "Hinv ?? /=".
-    iMod (compile_expr_execution_wpi' with "[$] [Hinv]") as "?"; [done|..].
-    { subst. by constructor. }
-    { iPoseProof Hwp as "Hwp". rewrite wp_heaplang_eq. by iApply "Hwp". }
-    iApply fupd_mask_intro; [done|]. by iIntros "?".
+  - move => ? ? Hval.
+    apply: (heaplang_soundness n). intros ? ?.
+    iDestruct (Hwp _ _) as "Hwp".
+    opose proof (execution_wpi _ _ _) as Had.
+    iIntros "Hinv Hs Hlc". iMod (Had with "Hs Hinv Hwp") as "Had"; eauto.
+    { rewrite Hval. apply tp_termination_TermRet. }
+    (* TODO: find a less hacky way to do this *)
+    simpl. iApply fupd_mask_intro; first done. iIntros "_".
+    by iApply step_fupdN_intro.
   - move => e2 _ /elem_of_list_lookup [? He2].
     destruct (decide (not_stuck e2 σ2)) as [?| Hstuck%not_not_stuck]; [done|].
     exfalso.
-    apply: (heaplang_soundness 0).
-    iIntros (? ?) "Hinv ?? /=".
-    iMod (compile_expr_execution_wpi' with "[$] [Hinv]") as "?"; [done|..].
-    { apply tp_termination_TermUb. eexists _, _. done. }
-    { iPoseProof Hwp as "Hwp". rewrite wp_heaplang_eq. by iApply "Hwp". }
+    apply: (heaplang_soundness n). intros ? ?.
+    iDestruct (Hwp _ _) as "Hwp".
+    opose proof (execution_wpi _ _ _) as Had.
+    iIntros "Hinv Hs". iMod (Had with "Hs Hinv Hwp") as "Had"; eauto.
+    { apply tp_termination_TermUb. econstructor. by eexists. }
     done.
 Qed.
